src/alt_Impl_appraisal.v
@@ -6,6 +6,8 @@ Require Import Impl_vm StAM. *)
 Require Import List.
 Import ListNotations.
 
+Require Import OptMonad.
+
 (*
 Definition am_add_trace (tr':list Ev) : AM_St -> AM_St :=
   fun '{| am_nonceMap := nm;
@@ -67,19 +69,63 @@ Admitted.
 Definition checkSig (e:EvidenceC) (p:Plc) (sig:BS) : BS.
 Admitted.
 
-Definition checkHash (e:Evidence) (p:Plc) (hash:BS) : BS.
+Definition checkHash (e:Evidence) (p:Plc) (hash:list BSV) : BS.
 Admitted.
 
+Definition peelBitsVval (e:EvidenceC) : option (BS*EvidenceC) :=
+  match e with
+  | PairBitsV (BitsV (bsval bs)) e' => Some (bs,e')
+  | _ => None
+  end.
+
+Definition peelBitsVhsh (e:EvidenceC) : option (list BSV*EvidenceC) :=
+  match e with
+  | PairBitsV (BitsV (bshsh ls)) e' => Some (ls,e')
+  | _ => None
+  end.
+    
+Definition peelPairBitsV (e:EvidenceC) : option (EvidenceC*EvidenceC) :=
+  match e with
+  | PairBitsV e1 e2 => ret (e1,e2)
+  | _ => None
+  end.
+    
 
     
-Fixpoint build_app_comp_ev (e:EvidenceC) (et:Evidence): EvidenceC :=
-  match (e,et) with
-  | (mtc,mt) => mtc
+Fixpoint build_app_comp_ev (e:EvidenceC) (et:Evidence): option EvidenceC :=
+  match et with
+  | mt => ret (BitsV (bsval 0))
               
-  | (uuc i args tpl tid bs e', uu i' args' tpl' tid' et') =>
-      uuc i' args' tpl' tid'
-          (checkASP i' args' tpl' tid' bs)
-          (build_app_comp_ev e' et')
+  | uu i' args' tpl' tid' et' =>
+    '(bs,e') <- peelBitsVval e ;;
+    res <- (build_app_comp_ev e' et') ;;
+    ret (PairBitsV (BitsV (bsval (checkASP i' args' tpl' tid' bs))) res)
+  | gg pi et' =>
+    '(bs,e') <- peelBitsVval e ;;
+    res <- (build_app_comp_ev e' et') ;;
+    ret (PairBitsV (BitsV (bsval (checkSig e' pi bs))) res)
+  | hh pi et' =>
+    (*'(bs,e') <- peelPairBitsV e ;; *)
+   
+    match e with
+    | BitsV (bshsh ls) =>
+       ret (BitsV (bsval (checkHash et' pi ls)))
+    | _ => None
+    end
+  | nn nid => ret (BitsV (bsval nid)) (* TODO: do checkNonce *)
+  | ss et1 et2 =>
+    '(e1,e2) <- peelPairBitsV e ;;
+      e1_res <- build_app_comp_ev e1 et1 ;;
+      e2_res <- build_app_comp_ev e2 et2 ;;
+      ret (PairBitsV e1_res e2_res)
+  | pp et1 et2 =>
+    '(e1,e2) <- peelPairBitsV e ;;
+      e1_res <- build_app_comp_ev e1 et1 ;;
+      e2_res <- build_app_comp_ev e2 et2 ;;
+      ret (PairBitsV e1_res e2_res)
+  end.
+
+(*
   | (ggc pi bs e', gg pi' et') =>
       ggc pi'
           (checkSig e' pi bs)
@@ -98,3 +144,4 @@ Fixpoint build_app_comp_ev (e:EvidenceC) (et:Evidence): EvidenceC :=
         
   | _ => mtc
   end.
+*)
